solution proposal for Rejecting_TM locale issue
omitting the name of the `sublocale` expression (`sublocale <locale> <item>` instead of `sublocale <name>: <locale> <item>`) allows using locale definitions inline
this seems to resolve most issues associated with the Rejecting_TM
rename the locale to "Rej_TM" to avoid the name conflict with the definition

papers/116_stefan_rass/TM.thy
@@ -567,48 +567,50 @@ end \<comment> \<open>context \<^locale>\<open>TM\<close>\<close>
 
 subsection\<open>Rejecting TM\<close>
 
-locale Rejecting_TM
+
+locale Rej_TM =
+  fixes \<Sigma> :: "'b::blank set"
+  assumes finite_alphabet: "finite \<Sigma>"
 begin
 
-definition "Rejecting_TM \<equiv> \<lparr>
-  tape_count = 1,
-  states = {1}::nat set,
-  start_state = 1,
-  final_states = {1},
-  accepting_states = {},
-  symbols = UNIV,
-  next_state = \<lambda>q w. 1,
-  next_action = \<lambda>q w. [Nop]
-\<rparr> :: (nat, 'b::{blank, finite}) TM"
+definition Rejecting_TM :: "(nat, 'b) TM"
+  where [simp]: "Rejecting_TM \<equiv> \<lparr>
+    tape_count = 1,
+    states = {1}::nat set,
+    start_state = 1,
+    final_states = {1},
+    accepting_states = {},
+    symbols = \<Sigma> \<union> {Bk},
+    next_state = \<lambda>q w. 1,
+    next_action = \<lambda>q w. [Nop]
+  \<rparr>"
 
-sublocale TM:
-  TM Rejecting_TM
-  unfolding Rejecting_TM_def
-  by (unfold_locales) simp_all
+sublocale TM "Rejecting_TM"
+  unfolding Rejecting_TM_def using finite_alphabet
+  by unfold_locales simp_all
 
 lemma rej_TM:
-  fixes w :: "'a::{finite, blank} list"
-  shows "TM.rejects w"
-  unfolding TM.rejects_def
+  assumes "set w \<subseteq> \<Sigma>"
+  shows "rejects w"
+  unfolding rejects_def
 proof
-  show "TM.wf_word w" unfolding Rejecting_TM_def by simp
+  show "wf_word w" using assms by auto
 next
-  show "TM.hoare_halt (TM.init w) (\<lambda>c. state c \<notin> accepting_states Rejecting_TM)"
+  let ?acc = "accepting_states Rejecting_TM"
+  show "hoare_halt (init w) (\<lambda>c. state c \<notin> ?acc)"
   proof
-    fix c0::"(nat, 'a) TM_config"
-    assume "TM.init w c0"
-    then have "state c0 = start_state (Rejecting_TM::(nat, 'a) TM)"
-      by (fact TM.init_state_start_state)
-    then have "TM.is_final ((TM.step^^0) c0)"
-      unfolding Rejecting_TM_def by simp
-    moreover have "accepting_states Rejecting_TM = {}"
-      unfolding Rejecting_TM_def by simp
-    ultimately show "\<exists>n. let cn = (TM.step ^^ n) c0 in TM.is_final cn \<and> state cn \<notin> accepting_states Rejecting_TM"
+    fix c0
+    assume "init w c0"
+    then have "state c0 = start_state Rejecting_TM" by (fact init_state_start_state)
+    then have "is_final ((step^^0) c0)" unfolding Rejecting_TM_def by simp
+    moreover have "?acc = {}" unfolding Rejecting_TM_def by simp
+    ultimately show "\<exists>n. let cn = (step ^^ n) c0 in is_final cn \<and> state cn \<notin> ?acc"
       using empty_iff by metis
   qed
 qed
 
-end \<comment> \<open>\<^locale>\<open>Rejecting_TM\<close>\<close>
+end \<comment> \<open>\<^locale>\<open>Rej_TM\<close>\<close>
+
 
 subsection\<open>(nat, nat) TM\<close>
 text \<open>Every well-formed TM is equivalent to some (nat, nat) TM\<close>
